extract/FileTest.v
@@ -1,0 +1,9 @@
+From SimpleIO Require Import
+     IO_Random.
+From FileSync Require Import
+     Execute.
+
+Definition run_test: io_unit :=
+  IO.unsafe_run' (ORandom.self_init tt;; fileTester).
+
+Separate Extraction run_test.
