theories/Execute.v
@@ -1,0 +1,119 @@
+From FileSync Require Export
+     Gen
+     Server
+     Semantics.
+From SimpleIO Require Export
+     IO_Random
+     IO_Sys
+     SimpleIO.
+From ITreeIO Require Export
+     ITreeIO.
+From Coq Require Export
+     ExtrOcamlBasic
+     ExtrOcamlIntConv
+     ExtrOcamlNativeString.
+Import
+  SumNotations
+  OSys.
+Open Scope sum_scope.
+
+Parameter ols   : string -> IO (list string).
+Parameter orm   : list string -> IO bool.
+Parameter omkdir: string -> IO bool.
+Extract Constant ols =>
+  "fun p k -> k (try FileUtil.ls p with 
+   _ -> prerr_endline ""ls: error""; [])".
+Extract Constant orm =>
+  "fun p k -> k (try FileUtil.rm ~recurse:true p; true with
+   | FileUtil.RmError str -> prerr_endline str; false
+   | _ -> prerr_endline ""rm: error""; false)".
+Extract Constant omkdir =>
+  "fun p k -> k (try FileUtil.mkdir p; true with
+   | FileUtil.MkdirError str -> prerr_endline str; false
+   | _ -> prerr_endline ""mkdir: error""; false)".
+Extract Inductive string => "string"
+[
+(* EmptyString *)
+"(* If this appears, you're using String internals. Please don't *)
+  """"
+"
+(* String *)
+"(* If this appears, you're using String internals. Please don't *)
+  (fun (c, s) -> String.make 1 c ^ s)
+"
+]
+"(* If this appears, you're using String internals. Please don't *)
+ (fun f0 f1 s ->
+    let l = String.length s in
+    if l = 0 then f0 () else f1 (String.get s 0) (String.sub s 1 (l-1)))
+".
+Extract Constant to_ostring => "(fun x -> x)".
+Extract Constant from_ostring => "(fun x -> x)".
+
+Parameter obasename: string -> string.
+Extract Constant obasename => "Filename.basename".
+
+Definition flatten: path -> string :=
+  String.concat "/".
+
+Definition read_file' (p: path) : IO content :=
+  cin <- open_in (flatten p);;
+  len <- in_channel_length cin;;
+  ostr <- really_input_string cin len;;
+  close_in_noerr cin;;
+  ret (from_ostring ostr).
+
+Definition read_file (p: path) : IO A :=
+  oc <- catch_exc (read_file' p);;
+  ret (if oc is Some c then Aread c else Ano).
+
+Definition write_file (p: path) (str: content) : IO A :=
+  ou <- catch_exc (cout <- open_out (flatten p);;
+                   output_string cout str;;
+                   close_out_noerr cout);;
+  ret (if ou is Some tt then Ayes else Ano).
+
+Arguments Observe__FromServer {_ _ _}.
+Arguments Observe__FromClient {_ _ _}.
+
+Definition runObserve {T} (oe: observeE Q A S T) : IO T :=
+  match oe in observeE _ _ _ T return _ T with
+  | Observe__FromServer QSync =>
+    command "unison -batch A B";; ret Ayes
+  | Observe__FromServer (QFile r f) =>
+    let base: path := if r is R1 then ["A"] else ["B"] in
+    tee $
+    match f with
+    | Fls    p   => Als ∘ map obasename <$> ols (flatten (base ++ p))
+    | Fread  p   => read_file (base ++ p)
+    | Fwrite p s => write_file (base ++ p) s
+    | Fmkdir p   => b <- omkdir (flatten (base ++ p));;
+                   ret (if b : bool then Ayes else Ano)
+    | Frm    p   => b <- orm [flatten (base ++ p)];;
+                   ret (if b : bool then Ayes else Ayes )
+    end
+  | Observe__FromClient s =>
+    tee $
+    let '(g, a, b) := s in
+    r <- io_choose [R1; R2];;
+    p <- gen_many 3 gen_string;;
+    c <- gen_string;;
+    io_choose [QSync;
+              QFile r (Fls p);
+              QFile r (Fread p);
+              QFile r (Fwrite p c);
+              QFile r (Fmkdir p);
+              QFile r (Frm p)]
+  end.
+
+Definition runO T (oe: oE Q A S T) : IO T :=
+  match oe with
+  | (oe|)        => runObserve oe
+  | (|Throw str) => failwith str
+  end.
+
+Definition fileServer   := serverOf qstep initS.
+Definition fileObserver := observe fileServer.
+Definition fileTester   :=
+  orm ["A"; "B"];; omkdir "A";; omkdir "B";; command "unison -batch A B";;
+  interp_io runO fileObserver.
