theories/Gen.v
@@ -1,0 +1,63 @@
+From ExtLib Require Export
+     Extras
+     Applicative
+     Functor
+     Monad.
+From SimpleIO Require Export
+     IO_Random
+     SimpleIO.
+From Ceres Require Export
+     CeresSerialize.
+From Coq Require Export
+     Basics
+     ExtrOcamlIntConv
+     String
+     List.
+Export
+  FunNotation
+  FunctorNotation
+  MonadNotation
+  ListNotations.
+Open Scope monad_scope.
+Open Scope string_scope.
+Open Scope program_scope.
+
+Definition tee {A} `{Serialize A} (io: IO A) : IO A :=
+  a <- io;;
+  prerr_endline (to_string a);;
+  ret a.
+
+Definition io_choose_ {A} (default : IO A) (l : list A) : IO A :=
+  match l with
+  | [] => default
+  | a :: _ =>
+    i <- nat_of_int <$> ORandom.int (int_of_nat (length l));;
+    ret (nth i l a)
+  end.
+
+Definition io_choose' {A} (l : list A) : IO (nat * A) :=
+  match l with
+  | [] => failwith "Cannot choose from empty list"
+  | a :: _ =>
+    i <- nat_of_int <$> ORandom.int (int_of_nat (length l));;
+    ret (i, nth i l a)
+  end.
+
+Definition io_choose {A} : list A -> IO A :=
+  fmap snd ∘ io_choose'.
+
+Definition io_or {A} (x y : IO A) : IO A :=
+  b <- ORandom.bool tt;;
+  if b : bool then x else y.
+
+Definition gen_string' : IO string :=
+  io_choose ["foo"; "bar"].
+
+Fixpoint gen_many {A} (n : nat) (ma : IO A) : IO (list A) :=
+  match n with
+  | O => ret []
+  | S n' => liftA2 cons ma $ io_or (ret []) (gen_many n' ma)
+  end.
+
+Definition gen_string : IO string :=
+  String.concat "." <$> gen_many 3 gen_string'.
